pipeline theorem complete

theories/Pipeline.v
@@ -19,6 +19,15 @@ Import PCUICTransform (template_to_pcuic_transform, pcuic_expand_lets_transform)
   shrinking of the global environment dependencies +
   the optimization that removes all pattern-matches on propositions. *)
 
+  Lemma All_sq {A} (P : A -> Type) l :
+    Forall (fun x => squash (P x)) l ->
+    squash (All P l).
+  Proof using Type.
+    induction 1.
+    - repeat econstructor.
+    - sq. now constructor.
+  Qed.
+  
 Import Transform.
 
 #[local] Arguments transform : simpl never. 
@@ -100,7 +109,7 @@ Proof.
   - unfold check_good_for_extraction. rtoProp. intros []. admit.
 Admitted.
 
-Obligation Tactic := try now program_simpl.
+#[local] Obligation Tactic := try now program_simpl.
 
 Program Definition enforce_extraction_conditions (efl := EWellformed.all_env_flags) `{Pointer} `{Heap} :
   t EAst.global_declarations EAst.global_declarations EAst.term EAst.term EAst.term
@@ -162,7 +171,7 @@ Proof.
   now rewrite -eq.
 Qed.
 
-Obligation Tactic := program_simpl.
+#[local] Obligation Tactic := program_simpl.
 
 Definition annotate_decl Γ (d : EAst.global_decl) :=
   match d with
@@ -292,14 +301,20 @@ Next Obligation.
     Unshelve. all: todo "global env".
 Qed.
 
+Program Definition verified_named_erasure_pipeline (efl := EWellformed.all_env_flags) `{Heap}:
+ Transform.t global_env_ext_map _ _ _ _ EWcbvEvalNamed.value 
+             PCUICTransform.eval_pcuic_program
+             (fun p v => ∥ EWcbvEvalNamed.eval p.1 [] p.2 v ∥) :=
+  verified_erasure_pipeline ▷
+  enforce_extraction_conditions ▷
+  implement_box_transformation ▷
+  name_annotation.
+
 Program Definition verified_malfunction_pipeline (efl := EWellformed.all_env_flags) `{Heap}:
  Transform.t global_env_ext_map _ _ _ _ SemanticsSpec.value 
              PCUICTransform.eval_pcuic_program
              (fun _ _ => True) :=
-  verified_erasure_pipeline ▷
-  enforce_extraction_conditions ▷
-  implement_box_transformation ▷
-  name_annotation ▷
+  verified_named_erasure_pipeline ▷
   compile_to_malfunction named_extraction_env_flags.
 Next Obligation.
   cbn. intros.
@@ -307,12 +322,39 @@ Next Obligation.
   eapply H1.
 Qed.
 
-Section malfunction_pipeline_theorem.
+
+Section compile_malfunction_pipeline.
 
   Local Existing Instance CanonicalHeap.
 
   Instance cf_ : checker_flags := extraction_checker_flags.
   Instance nf_ : PCUICSN.normalizing_flags := PCUICSN.extraction_normalizing.
+
+  Variable HP : Pointer.
+  Variable HH : Heap.
+
+  Variable Σ : global_env_ext_map.
+  Variable t : PCUICAst.term.
+  Variable T : PCUICAst.term.
+
+  Variable HΣ : PCUICTyping.wf_ext Σ.
+  Variable expΣ : PCUICEtaExpand.expanded_global_env Σ.1.
+  Variable expt : PCUICEtaExpand.expanded Σ.1 [] t.
+  Variable typing : PCUICTyping.typing Σ [] t T.
+
+  Variable Normalisation : forall Σ0 : PCUICAst.PCUICEnvironment.global_env_ext,
+  PCUICTyping.wf_ext Σ0 -> PCUICSN.NormalizationIn Σ0.
+
+  Definition compile_malfunction_pipeline := transform verified_malfunction_pipeline (Σ, t) (precond _ _ _ _ expΣ expt typing _).
+  
+End compile_malfunction_pipeline. 
+
+Section malfunction_pipeline_theorem.
+
+  Local Existing Instance CanonicalHeap.
+
+  Instance cf__ : checker_flags := extraction_checker_flags.
+  Instance nf__ : PCUICSN.normalizing_flags := PCUICSN.extraction_normalizing.
 
   Variable HP : Pointer.
   Variable HH : Heap.
@@ -332,63 +374,44 @@ Section malfunction_pipeline_theorem.
 
   Variable typing : PCUICTyping.typing Σ [] t (PCUICAst.mkApps (PCUICAst.tInd i u) args).
 
-  Variable fo : forall i, @PCUICFirstorder.firstorder_ind Σ (PCUICFirstorder.firstorder_env Σ) i.
+  Variable fo : @PCUICFirstorder.firstorder_ind Σ (PCUICFirstorder.firstorder_env Σ) i.
 
   Variable noParam : forall i mdecl, lookup_env Σ i = Some (InductiveDecl mdecl) -> ind_npars mdecl = 0. 
 
   Variable Normalisation : forall Σ0 : PCUICAst.PCUICEnvironment.global_env_ext,
   PCUICTyping.wf_ext Σ0 -> PCUICSN.NormalizationIn Σ0.
 
-  Lemma precond_ : pre verified_erasure_pipeline (Σ, t).
-  Proof.
-    eapply precond; eauto.
-  Defined.
+  Let Σ_t := (compile_malfunction_pipeline _ _ _ _ _ _ expΣ expt typing _).1.
+  Let t_t := (compile_malfunction_pipeline _ _ _ _ _ _ expΣ expt typing _).2.
 
-  Let Σ_t := (transform verified_malfunction_pipeline (Σ, t) precond_).1.
+  Variable Heval : ∥PCUICWcbvEval.eval Σ t v∥.
 
-  Program Definition Σ_b `{EWellformed.EEnvFlags} := (transform (verified_erasure_pipeline ▷  enforce_extraction_conditions ▷ implement_box_transformation ▷ name_annotation) (Σ, t) precond_).1.
+  Let Σ_v := (transform verified_named_erasure_pipeline (Σ, v) (precond2 _ _ _ _ expΣ expt typing _ _ Heval)).1.
+  Let Σ_t' := (transform verified_named_erasure_pipeline (Σ, t) (precond _ _ _ _ expΣ expt typing _)).1.
 
-  Let t_t := (transform verified_malfunction_pipeline (Σ, t) precond_).2.
-
-  Fixpoint compile_value_mf_acc (Σb : list (Kernames.kername × EAst.global_decl)) (t : PCUICAst.term) (acc : list SemanticsSpec.value) : SemanticsSpec.value :=
+  Fixpoint compile_value_mf_aux Σb (t : EAst.term) : SemanticsSpec.value :=
     match t with
-    | PCUICAst.tApp f a => compile_value_mf_acc Σb f (compile_value_mf_acc Σb a [] :: acc)
-    | PCUICAst.tConstruct i n _ => 
-    match acc with
-    | [] =>
-        match lookup_constructor_args Σb i with
-        | Some num_args =>
-            let num_args_until_m := firstn n num_args in
-            let index :=
-              #|filter
-                  (fun x : nat =>
-                   match x with
-                   | 0 => true
-                   | S _ => false
-                   end) num_args_until_m| in
-            value_Int (Malfunction.Int, Z.of_nat index)
+    | EAst.tConstruct i m [] =>
+      match lookup_constructor_args Σb i with
+        | Some num_args => 
+            let num_args_until_m := firstn m num_args in
+            let index := #| filter (fun x => match x with 0 => true | _ => false end) num_args_until_m| in
+            SemanticsSpec.value_Int (Malfunction.Int, BinInt.Z.of_nat index)
         | None => fail "inductive not found"
-        end
-    | _ :: _ =>
-        match lookup_constructor_args Σb i with
-        | Some num_args =>
-            let num_args_until_m := firstn n num_args in
-            let index :=
-              #|filter
-                  (fun x : nat =>
-                   match x with
-                   | 0 => false
-                   | S _ => true
-                   end) num_args_until_m| in
-            Block
-              (utils_array.int_of_nat index, acc)
+      end
+    | EAst.tConstruct i m args =>
+      match lookup_constructor_args Σb i with
+        | Some num_args => 
+            let num_args_until_m := firstn m num_args in
+            let index := #| filter (fun x => match x with 0 => false | _ => true end) num_args_until_m| in
+            Block (utils_array.int_of_nat index, map (compile_value_mf_aux Σb) args)
         | None => fail "inductive not found"
-        end
-    end
+      end
     | _ => not_evaluated
     end.
-    
-  Definition compile_value_mf Σb t := compile_value_mf_acc Σb t [].
+
+  Definition compile_value_mf Σ Σb t :=   
+    compile_value_mf_aux Σb (compile_value_box (PCUICExpandLets.trans_global_env Σ) t []).
 
   Lemma compile_value_box_mkApps Σb i0 n ui args0: 
     compile_value_box Σb (PCUICAst.mkApps (PCUICAst.tConstruct i0 n ui) args0) [] =
@@ -402,46 +425,21 @@ Section malfunction_pipeline_theorem.
       do 2 f_equal. repeat rewrite map_app. cbn. now repeat rewrite <- app_assoc.
   Qed.
 
-  Lemma compile_value_mf_mkApps Σb i0 n ui args0: 
-    compile_value_mf Σb (PCUICAst.mkApps (PCUICAst.tConstruct i0 n ui) args0) =
-    compile_value_mf_acc Σb (PCUICAst.tConstruct i0 n ui) (map (fun v => compile_value_mf Σb v) args0).
-  Proof.
-    unfold compile_value_mf. rewrite <- (app_nil_r (map _ _)). 
-    generalize (@nil SemanticsSpec.value) at 1 3. induction args0 using rev_ind; cbn.
-    - intro l; case_eq l; intros; destruct lookup_constructor_args; eauto.
-    - intros l. rewrite PCUICAstUtils.mkApps_nonempty; eauto.
-      cbn. rewrite removelast_last last_last. rewrite IHargs0. cbn. 
-      repeat rewrite map_app; cbn; repeat rewrite <- app_assoc.
-      destruct lookup_constructor_args; eauto.
-  Qed.
-
-  Fixpoint eval_fo kn (t: EAst.term) : EWcbvEvalNamed.value :=   
+  Fixpoint eval_fo (t: EAst.term) : EWcbvEvalNamed.value :=   
     match t with 
-      | EAst.tConstruct ind c args => vConstruct ind c (map (eval_fo kn) args)
-      | _ => vConstruct kn 0 []
+      | EAst.tConstruct ind c args => vConstruct ind c (map eval_fo args)
+      | _ => vClos "" (EAst.tVar "error") []
     end. 
 
-  Lemma All_sq {A} (P : A -> Type) l :
-    Forall (fun x => squash (P x)) l ->
-    squash (All P l).
-  Proof using Type.
-    induction 1.
-    - repeat econstructor.
-    - sq. now constructor.
-  Qed.
-
-  Lemma compile_value_eval_fo_repr {Henvflags:EWellformed.EEnvFlags} kn : 
+  Lemma compile_value_eval_fo_repr {Henvflags:EWellformed.EEnvFlags} : 
     PCUICFirstorder.firstorder_value Σ [] t ->
     let v := compile_value_box (PCUICExpandLets.trans_global_env Σ) t [] in
-    ∥ EWcbvEvalNamed.represents_value (eval_fo kn v) v∥.
+    ∥ EWcbvEvalNamed.represents_value (eval_fo v) v∥.
   Proof.
-    intro H. cbn.
-    unfold precond_ in *. clear Σ_t t_t.
+    intro H. cbn. clear Σ_t.
     pattern t.
     refine (PCUICFirstorder.firstorder_value_inds _ _ _ _ _ H). 
-    intros.
-    rewrite compile_value_box_mkApps.
-    cbn.
+    intros. rewrite compile_value_box_mkApps. cbn.
     eapply PCUICValidity.validity in X. eapply PCUICInductiveInversion.wt_ind_app_variance in X as [mdecl [? ?]].  
     unfold pcuic_lookup_inductive_pars. unfold lookup_inductive,lookup_inductive_gen,lookup_minductive_gen in e.
     rewrite PCUICExpandLetsCorrectness.trans_lookup. specialize (noParam (inductive_mind i0)). 
@@ -456,107 +454,6 @@ Section malfunction_pipeline_theorem.
     solve_all.
   Qed.
 
-  Lemma compile_value_eval_fo {Henvflags:EWellformed.EEnvFlags} kn : 
-    PCUICFirstorder.firstorder_value Σ [] t ->
-    let v := compile_value_box (PCUICExpandLets.trans_global_env Σ) t [] in
-    ∥EWcbvEvalNamed.eval Σ_b [] v (eval_fo kn v)∥.
-  Proof.
-    intro H. unfold Σ_b. repeat destruct_compose; intros. cbn.
-    unfold precond_ in *. clear Σ_t t_t. 
-    revert typing expt H0 H1 H2.
-    refine (PCUICFirstorder.firstorder_value_inds _ _ (fun t => forall (typing : Σ;;; [] |- t : mkApps (tInd i u) args)
-    (expt : PCUICEtaExpand.expanded Σ.1 [] t)
-    (H0 : pre enforce_extraction_conditions
-            (transform verified_erasure_pipeline (Σ, t)
-               (precond Σ HΣ expΣ t expt i u args typing Normalisation)))
-    (H1 : pre implement_box_transformation
-            (transform enforce_extraction_conditions
-               (transform verified_erasure_pipeline (Σ, t)
-                  (precond Σ HΣ expΣ t expt i u args typing Normalisation)) H0))
-    (H2 : pre name_annotation
-            (transform implement_box_transformation
-               (transform enforce_extraction_conditions
-                  (transform verified_erasure_pipeline (
-                     Σ, t) (precond Σ HΣ expΣ t expt i u args typing Normalisation))
-                  H0) H1)),
-  ∥ EWcbvEvalNamed.eval
-      (transform name_annotation
-         (transform implement_box_transformation
-            (transform enforce_extraction_conditions
-               (transform verified_erasure_pipeline (Σ, t)
-                  (precond Σ HΣ expΣ t expt i u args typing Normalisation)) H0) H1)
-         H2).1 [] (compile_value_box (PCUICExpandLets.trans_global_env Σ.1) t [])
-      (eval_fo kn (compile_value_box (PCUICExpandLets.trans_global_env Σ.1) t [])) ∥) _ _ H); intros; clear H.
-    rewrite compile_value_box_mkApps.
-    eapply Forall_All in H1. cbn. pose proof (X' := X).
-    eapply PCUICValidity.validity in X. eapply PCUICInductiveInversion.wt_ind_app_variance in X as [mdecl [? ?]].  
-    unfold pcuic_lookup_inductive_pars. unfold lookup_inductive,lookup_inductive_gen,lookup_minductive_gen in e.
-    rewrite PCUICExpandLetsCorrectness.trans_lookup. specialize (noParam (inductive_mind i0)). 
-    case_eq (lookup_env Σ (inductive_mind i0)); cbn.  
-    2: { intro neq. rewrite neq in e. inversion e. }
-    intros ? Heq. rewrite Heq in e. rewrite Heq. destruct g; cbn; [inversion e |]. destruct nth_error; inversion e; subst; cbn.  
-    assert (ind_npars m = 0) by eauto. rewrite H. rewrite skipn_0.
-    eapply PCUICValidity.inversion_mkApps in X' as [A [X' ?]].  
-    eapply PCUICInversion.inversion_Construct in X' as [? [? [? [? [? [? ?]]]]]]; eauto.
-    eapply map_squash. intro. econstructor. 3: exact X. 1-2: admit. 
-    induction H1; cbn. econstructor; eauto. inversion t0; subst; clear t0. inversion H0; subst.
-(*    specialize (p _ _ _).    
-    eapply map_squash. intro; econstructor. [apply p | eauto].
-    eapply IHAll; eauto. inversion H0; eauto. }
-    eapply declared_constructor_to_gen in d. 
-    rewrite /declared_constructor_gen /declared_inductive_gen /declared_minductive_gen in d.
-    unfold Σ_b. repeat destruct_compose; intros. 
-    rewrite /EGlobalEnv.lookup_constructor /EGlobalEnv.lookup_inductive /EGlobalEnv.lookup_minductive.
-    rewrite EExtends. lookup_env_In. 
-    rewrite <- EEnvMap.GlobalContextMap.lookup_env_spec.
-    cbn. 
-    destruct EGlobalEnv.lookup_env eqn:Henv => //=.
-    destruct g => //.
-    eapply he in declm; tea. subst m.
-    rewrite nth_error_map decli /=.
-    rewrite nth_error_map declc /=. intuition congruence.
-    unfold Σ_b. repeat destruct_compose; intros.
-    
-
-      
-      
-    
-    
-    (* revert typing Σ_b.  refine (PCUICFirstorder.firstorder_value_inds _ _ (fun p => let v := compile_value_box (PCUICExpandLets.trans_global_env Σ) p [] in *)
-    (* ∥EWcbvEvalNamed.eval Σ_b [] v (eval_fo kn v)∥) _ _ H); intros; clear H.  *)
-    (* unfold v0. clear v0. rewrite compile_value_box_mkApps. *)
-    (* eapply Forall_All in H1. cbn. pose proof (X' := X). *)
-    (* eapply PCUICValidity.validity in X. eapply PCUICInductiveInversion.wt_ind_app_variance in X as [mdecl [? ?]].   *)
-    (* unfold pcuic_lookup_inductive_pars. unfold lookup_inductive,lookup_inductive_gen,lookup_minductive_gen in e. *)
-    (* rewrite PCUICExpandLetsCorrectness.trans_lookup. specialize (noParam (inductive_mind i0)).  *)
-    (* case_eq (lookup_env Σ (inductive_mind i0)); cbn.   *)
-    (* 2: { intro neq. rewrite neq in e. inversion e. } *)
-    (* intros ? Heq. rewrite Heq in e. rewrite Heq. destruct g; cbn; [inversion e |]. destruct nth_error; inversion e; subst; cbn.   *)
-    (* assert (ind_npars m = 0) by eauto. rewrite H. rewrite skipn_0. *)
-    (* eapply PCUICValidity.inversion_mkApps in X' as [A [X' ?]].   *)
-    (* eapply PCUICInversion.inversion_Construct in X' as [? [? [? [? [? [? ?]]]]]]; eauto. *)
-    (* eapply map_squash. intro. econstructor. 3: exact X. *)
-    (* 3 :{ clear t0.  induction H1; cbn. econstructor; eauto. *)
-    (* cbn in p0. destruct p0 as [p0]. eapply map_squash. intro; econstructor; [exact p0 | eauto]. *)
-    (* eapply IHAll; eauto. inversion H0; eauto. } *)
-    (* eapply declared_constructor_to_gen in d.  *)
-    (* rewrite /declared_constructor_gen /declared_inductive_gen /declared_minductive_gen in d. *)
-    (* unfold Σ_b. repeat destruct_compose; intros.  *)
-    (* rewrite /EGlobalEnv.lookup_constructor /EGlobalEnv.lookup_inductive /EGlobalEnv.lookup_minductive. *)
-    (* rewrite EExtends. lookup_env_In.  *)
-    (* rewrite <- EEnvMap.GlobalContextMap.lookup_env_spec. *)
-    (* cbn.  *)
-    (* destruct EGlobalEnv.lookup_env eqn:Henv => //=. *)
-    (* destruct g => //. *)
-    (* eapply he in declm; tea. subst m. *)
-    (* rewrite nth_error_map decli /=. *)
-    (* rewrite nth_error_map declc /=. intuition congruence. *)
-    (* unfold Σ_b. repeat destruct_compose; intros. *)
-    
-
-    (* 2: { rewrite map_length.  } *) *)
-  Admitted.
-
   From Equations Require Import Equations.
 
   Lemma implement_box_fo {Henvflags:EWellformed.EEnvFlags} p : 
@@ -566,85 +463,169 @@ Section malfunction_pipeline_theorem.
   Proof.
   intro H. refine (PCUICFirstorder.firstorder_value_inds _ _ (fun p => let v := compile_value_box (PCUICExpandLets.trans_global_env Σ) p [] in
   v = EImplementBox.implement_box v) _ _ H); intros. revert v0. 
-  rewrite compile_value_box_mkApps. intro v0. cbn in v0. destruct pcuic_lookup_inductive_pars; eauto. 
-  assert (n0 = 0) by admit. subst. revert v0; rewrite skipn_0. set (map _ _). simpl. rewrite EImplementBox.implement_box_unfold_eq. simpl.
+  rewrite compile_value_box_mkApps. intro v0. cbn in v0. revert v0.
+  unfold pcuic_lookup_inductive_pars. rewrite PCUICExpandLetsCorrectness.trans_lookup.
+  case_eq (lookup_env Σ (inductive_mind i0)).
+  2: { intro Hlookup; now rewrite Hlookup. }       
+  intros ? Hlookup; rewrite Hlookup. destruct g; eauto; simpl.
+  specialize (noParam (inductive_mind i0)). assert (ind_npars m = 0) by eauto. rewrite H3. 
+  rewrite skipn_0. set (map _ _). simpl. rewrite EImplementBox.implement_box_unfold_eq. simpl.
   f_equal. erewrite MCList.map_InP_spec. clear -H1. unfold l; clear l. induction H1; eauto. simpl. f_equal; eauto.
-  Admitted.
+  Qed. 
         
-  Lemma represent_value_eval_fo p kn : 
+  Lemma represent_value_eval_fo p : 
     PCUICFirstorder.firstorder_value Σ [] p ->
     let v := compile_value_box (PCUICExpandLets.trans_global_env Σ) p [] in
-    forall v', represents_value v' v -> v' = eval_fo kn v.
+    forall v', represents_value v' v -> v' = eval_fo v.
   Proof.
     intro H. refine (PCUICFirstorder.firstorder_value_inds _ _ (fun p => let v := compile_value_box (PCUICExpandLets.trans_global_env Σ) p [] in
-    forall v', represents_value v' v -> v' = eval_fo kn v) _ _ H); intros. revert H3. 
+    forall v', represents_value v' v -> v' = eval_fo v) _ _ H); intros. revert H3. 
     unfold v0. clear v0. rewrite compile_value_box_mkApps.
-    eapply Forall_All in H1. cbn. destruct pcuic_lookup_inductive_pars; [| admit].
-    assert (n0 = 0) by admit. subst. rewrite skipn_0. cbn. inversion 1; subst; eauto. clear H3. 
-    f_equal. clear X H0 H2. revert vs H6. induction H1; cbn; inversion 1; f_equal; subst. 
+    eapply Forall_All in H1. cbn.
+    unfold pcuic_lookup_inductive_pars. rewrite PCUICExpandLetsCorrectness.trans_lookup.
+    case_eq (lookup_env Σ (inductive_mind i0)).
+    2: { intro Hlookup; now rewrite Hlookup. }
+    intros ? Hlookup; rewrite Hlookup. destruct g; eauto; simpl.
+    { inversion 1. }
+    specialize (noParam (inductive_mind i0)). assert (ind_npars m = 0) by eauto. rewrite H3. 
+    rewrite skipn_0. inversion 1; subst; eauto. clear H3 H4. 
+    f_equal. clear X H0 H2. revert vs H7. induction H1; cbn; inversion 1; f_equal; subst. 
     - eapply p0; eauto.
     - eapply IHAll; eauto.
-  Admitted. 
+  Qed.
 
-  Lemma compile_value_mf_eq {Henvflags: EWellformed.EEnvFlags} p kn : 
+  Definition compile_named_value p := eval_fo (compile_value_box (PCUICExpandLets.trans_global_env Σ) p []).
+
+  Opaque compose.   
+
+  Lemma compile_value_mf_eq {Henvflags: EWellformed.EEnvFlags} p : 
     PCUICFirstorder.firstorder_value Σ [] p ->
-    let v := compile_value_box (PCUICExpandLets.trans_global_env Σ) p [] in
-    compile_value_mf Σ_b p = compile_value Σ_b (eval_fo kn v).
+    compile_value_mf Σ Σ_v p = compile_value Σ_v (compile_named_value p).
   Proof.
-    intros H. refine (PCUICFirstorder.firstorder_value_inds _ _ (fun p => let v := compile_value_box (PCUICExpandLets.trans_global_env Σ) p [] in
-    compile_value_mf Σ_b p = compile_value Σ_b (eval_fo kn v)) _ _ H).
-    intros. rewrite compile_value_mf_mkApps. unfold v0. clear v0. rewrite compile_value_box_mkApps.    
-    clear H. cbn. unfold pcuic_lookup_inductive_pars. 
-    destruct PCUICAst.PCUICEnvironment.lookup_env ; [|admit].
-    destruct g ; [admit|].
-    assert ((PCUICAst.PCUICEnvironment.ind_npars m) = 0) by admit. rewrite H. rewrite skipn_0. cbn. 
-    destruct lookup_constructor_args. 2: { clear; destruct map; destruct map; eauto. }
+    intros H. refine (PCUICFirstorder.firstorder_value_inds _ _ 
+      (fun p => compile_value_mf Σ Σ_v p = compile_value Σ_v (compile_named_value p)) _ _ H).
+    unfold compile_named_value.
+    intros. unfold compile_value_mf. repeat rewrite compile_value_box_mkApps. 
+    clear H. cbn. specialize (noParam (inductive_mind i0)). 
+    unfold pcuic_lookup_inductive_pars. rewrite PCUICExpandLetsCorrectness.trans_lookup.
+    eapply PCUICValidity.validity in X. eapply PCUICInductiveInversion.wt_ind_app_variance in X as [mdecl [? _]].  
+    unfold lookup_inductive,lookup_inductive_gen,lookup_minductive_gen in e.
+    destruct lookup_env; cbn; try inversion e.
+    destruct g; cbn; try inversion e. 
+    assert (Hnpars: ind_npars m = 0) by eauto. rewrite Hnpars. 
+    rewrite skipn_0. destruct lookup_constructor_args; cbn.
+    2: { destruct map; eauto. }
     destruct args0; cbn; eauto.
     repeat f_equal; inversion H1; subst; clear H1; eauto.
     repeat rewrite map_map. eapply map_ext_Forall; eauto.
-  Admitted. 
+  Qed. 
     
-  Variable Heval : ∥PCUICWcbvEval.eval Σ t v∥.
-
   Variables (Σ' : _) (Henvflags:EWellformed.EEnvFlags)  (HΣ' : (forall (c : Kernames.kername) (decl : EAst.constant_body) 
                                (body : EAst.term) (v : EWcbvEvalNamed.value),
-                                EGlobalEnv.declared_constant Σ_b c decl ->
+                                EGlobalEnv.declared_constant Σ_t' c decl ->
                                 EAst.cst_body decl = Some body ->
-                                EWcbvEvalNamed.eval Σ_b [] body v ->
-                                In (Kernames.string_of_kername c, compile_value Σ_b v) Σ')).
+                                EWcbvEvalNamed.eval Σ_t' [] body v ->
+                                In (Kernames.string_of_kername c, compile_value Σ_t' v) Σ')).
 
   Variable (Haxiom_free : Extract.axiom_free Σ).
 
+  Lemma verified_malfunction_pipeline_lookup (efl := extraction_env_flags)  {has_rel : has_tRel} {has_box : has_tBox} 
+    kn g : 
+    EGlobalEnv.lookup_env Σ_v kn = Some g ->
+    EGlobalEnv.lookup_env Σ_t' kn = Some g. 
+  Proof.
+    unfold Σ_t', Σ_v. unfold verified_named_erasure_pipeline.
+    repeat (destruct_compose; intro). 
+    unfold transform at 1 3; cbn -[transform].
+    repeat (destruct_compose; intro). 
+    unfold transform at 1 3; cbn -[transform].
+    repeat (destruct_compose; intro). 
+    unfold transform at 1 3; cbn -[transform].
+    intro Hlookup.
+    rewrite lookup_env_annotate. rewrite lookup_env_annotate in Hlookup.  
+    rewrite lookup_env_implement_box. rewrite lookup_env_implement_box in Hlookup.
+    case_eq (EGlobalEnv.lookup_env (transform verified_erasure_pipeline (Σ, v)
+               (precond2 Σ t (mkApps (tInd i u) args) HΣ expΣ expt typing Normalisation v Heval)).1 kn).
+    2: { intros He. rewrite He in Hlookup; inversion Hlookup. }
+    intros ? Heq. rewrite Heq in Hlookup. cbn in Hlookup. 
+    eapply extends_lookup in Heq. rewrite Heq. eauto.
+    2: { eapply verified_erasure_pipeline_extends; eauto. }
+    epose proof (correctness _ _ H4). cbn in H5. now destruct H5.
+  Qed.
 
-  Lemma verified_malfunction_pipeline_theorem h :
-    ∥ SemanticsSpec.eval Σ' (fun _ => fail "notfound") h t_t h (compile_value_mf Σ_b v)∥.
+  Lemma verified_malfunction_pipeline_compat p (efl := extraction_env_flags) {has_rel : has_tRel} {has_box : has_tBox} 
+    : firstorder_evalue_block Σ_v p -> compile_value Σ_t' (eval_fo p) = compile_value Σ_v (eval_fo p).
+  Proof.
+    intros H. eapply firstorder_evalue_block_elim with (P := fun p => compile_value Σ_t' (eval_fo p) = compile_value Σ_v (eval_fo p)); [|eauto] ; intros. 
+    cbn. set (precond2 _ _ _ _ _ _ _ _ _ _) in Σ_v. unfold EGlobalEnv.lookup_constructor_pars_args in H0. cbn in H0.  
+    unfold lookup_constructor_args, EGlobalEnv.lookup_inductive. cbn.
+    case_eq (EGlobalEnv.lookup_env Σ_v (inductive_mind i0)).
+    2:{ intro HNone. rewrite HNone in H0; inversion H0. } 
+    intros ? HSome. rewrite HSome in H0; cbn in H0.
+    eapply verified_malfunction_pipeline_lookup in HSome; eauto. 
+    rewrite HSome.
+    destruct args0; cbn in *.  
+    { destruct g; cbn; eauto. }
+    { destruct g; cbn; [eauto|]. 
+      destruct (nth_error _ _); cbn; [|eauto].
+      inversion H2. subst. destruct H5.   
+      enough (map (compile_value Σ_t') (map eval_fo args0) = map (compile_value Σ_v) (map eval_fo args0)).
+      { now destruct H3. }
+      { clear - H6. induction H6; cbn. eauto. now destruct H, IHForall. } 
+    }
+    Unshelve. all: eauto. 
+  Qed. 
+
+  Lemma verified_malfunction_pipeline_theorem h (efl := extraction_env_flags) {has_rel : has_tRel} {has_box : has_tBox} :
+    ∥ SemanticsSpec.eval Σ' (fun _ => fail "notfound") h t_t h (compile_value_mf Σ Σ_v v)∥.
   Proof.
     unshelve epose proof (verified_erasure_pipeline_theorem _ _ _ _ _ _ _ _ _ _ _ _ _ Heval); eauto.
-    erewrite compile_value_mf_eq with (kn:=i). 
-    2: { eapply fo_v; eauto. }
-    unfold t_t, verified_malfunction_pipeline. sq. repeat destruct_compose; intros.
-    unfold compile_to_malfunction. unfold transform at 1. unfold compile_program. 
-    cbn. unfold Σ_b in *. revert HΣ'. repeat destruct_compose; intros.
-    (* YF: Had to comment this out because the apply is looping *)
-    (* eapply compile_correct with (Γ := []). intros.  *) 
-    (* - admit. (* bounds stuff *)  *)
-    (* - eauto.  *)
-    (* - eauto. *)
-    (* - cbn in H0, H1, H2, H3, H4. unfold name_annotation. unfold transform at 1 4. cbn.  *)
-    (*   epose proof (eval_to_eval_named_full _ _ _ _ _) as [? [? ?]]. *)
-    (*   5: { eapply represent_value_eval_fo in r. rewrite r in e. eapply e. eapply fo_v; eauto. } *)
-    (*   { admit. } *)
-    (*   { admit. } *)
-    (*   { rewrite implement_box_fo. eapply fo_v; eauto. eapply EImplementBox.implement_box_eval. 1-6: admit. *)
-    (*     eapply H. } *)
-    (*   admit.  *)
-  Admitted.
+    rewrite compile_value_mf_eq. 
+    { eapply fo_v; eauto. }
+    unfold t_t, compile_malfunction_pipeline, verified_malfunction_pipeline, verified_named_erasure_pipeline in *. revert HΣ'.
+    repeat destruct_compose ; intros.
+    unfold compile_to_malfunction. unfold transform at 1. simpl.
+    unshelve epose proof (Himpl := implement_box_transformation.(preservation) _ _ _ _); try eapply H1; eauto.
+    destruct Himpl as [? [Himpl_eval Himpl_obs]].
+    unfold obseq in Himpl_obs. simpl in Himpl_obs. rewrite Himpl_obs in Himpl_eval.
+    unshelve epose proof (Hname := name_annotation.(preservation) _ _ _ _);  try eapply H2; eauto.
+    { rewrite Himpl_obs; eauto. }
+    destruct Hname as [? [Hname_eval Hname_obs]]. simpl in *. sq.
+    unfold compile_named_value. rewrite <- verified_malfunction_pipeline_compat.
+    2-3: eauto. 
+    2: { unfold Σ_v. repeat destruct_compose ; intros.
+         unfold transform at 1; cbn -[transform]. 
+         unfold transform at 1; cbn -[transform].
+         unfold transform at 1; cbn -[transform].
+         unshelve epose proof (verified_erasure_pipeline_firstorder_evalue_block _ _ _ _ _ _ _ _ _ _ typing _ _ _); eauto.
+       }
+    unfold Σ_t'. repeat destruct_compose ; intros. 
+    eapply compile_correct with (Γ := []); intros.
+    - todo "bounds stuff". 
+    - eauto.  
+    - revert HΣ'. unfold Σ_t'. repeat destruct_compose ; intros. eauto. 
+    - rewrite Himpl_obs in Hname_obs. 
+      rewrite <- implement_box_fo in Hname_obs. 2: { eapply fo_v; eauto. }
+      eapply represent_value_eval_fo in Hname_obs. 2: { eapply fo_v; eauto. }
+      unfold compile_named_value. rewrite <- Hname_obs. exact Hname_eval.
+  Qed. 
 
-  (* Lemma verified_erasure_pipeline_lambda : *)
-  (*   PCUICAst.isLambda t -> EAst.isLambda t_t. *)
-  (* Proof. *)
-  (*   unfold t_t. clear. *)
-  (* Admitted. *)
+  Lemma verified_named_erasure_pipeline_fo :
+    firstorder_evalue_block Σ_v (compile_value_box Σ v []).
+  Proof.
+    unfold Σ_v, verified_named_erasure_pipeline.
+    repeat (destruct_compose; simpl; intro).
+    unshelve epose proof ErasureCorrectness.verified_erasure_pipeline_firstorder_evalue_block _ _ _ _ _ _ _ _ _ _ typing _ _ _; eauto.
+    assert (Hexpand: PCUICExpandLets.trans_global_env Σ = Σ) by todo "expand".
+    rewrite Hexpand in H2. set (v' := compile_value_box _ _ _) in *. clearbody v'.
+    clear -H2. eapply firstorder_evalue_block_elim; eauto. clear. intros; econstructor; eauto. 
+    clear -H. cbn in *. rewrite lookup_env_annotate lookup_env_implement_box.
+    unfold enforce_extraction_conditions. unfold transform at 1.
+    destruct EGlobalEnv.lookup_env; [|inversion H].
+    destruct g; inversion H; subst; eauto.   
+  Qed.    
+    
+  Transparent compose. 
 
 End malfunction_pipeline_theorem.
 
